incorporated simulation optimization for büchi complementation

thys/Buchi_Complementation/code/Complementation.sml
@@ -1,28 +1,8 @@
 open Complementation
+open Automaton
 
-fun nth l 0 = hd l
-  | nth l n = nth (tl l) (n - 1)
-
-fun getParameterString n default =
-	if length (CommandLine.arguments ()) <= n
-	then default
-	else nth (CommandLine.arguments ()) n
-
-fun getParameterInteger n default =
-	if length (CommandLine.arguments ()) <= n
-	then default
-	else
-		case Int.fromString (nth (CommandLine.arguments ()) n)
-		of SOME k => k
-		 | NONE => default
-
-fun naturalNumbers 0 = []
-  | naturalNumbers n = naturalNumbers (n - 1) @ [n - 1]
-
-fun run_test n =
+val _ =
 (
-	print (Int.toString (integer_of_nat (test n)) ^ "\n");
+	print (Int.toString (integer_of_nat (test automaton)) ^ "\n");
 	print (Statistics.pretty_stats (Statistics.get_active_stats ()) ^ "\n")
 )
-
-val _ = run_test (nat_of_integer (getParameterInteger 0 4))
