thys/Buchi_Complementation/Complementation_Final.thy
@@ -7,41 +7,6 @@ imports
   "HOL-Library.Permutation"
 begin
 
-  lemma complement_3_finite[simp]:
-    assumes "finite (nodes A)"
-    shows "finite (nodes (complement_3 A))"
-  proof -
-    have "(nodes (complement_3 A), nodes (complement_2 A)) \<in> \<langle>Id\<rangle> set_rel"
-      using complement_3_refine by parametricity auto
-    also have "(nodes (complement_2 A), nodes (complement_1 A)) \<in> \<langle>Id\<rangle> set_rel"
-      using complement_2_refine by parametricity auto
-    also have "(nodes (complement_1 A), nodes (complement A)) \<in> \<langle>cs_rel\<rangle> set_rel"
-      using complement_1_refine by parametricity auto
-    finally have 1: "(nodes (complement_3 A), nodes (complement A)) \<in> \<langle>cs_rel\<rangle> set_rel" by simp
-    have "finite (nodes (complement A))" using complement_finite assms(1) by this
-    then show "finite (nodes (complement_3 A))"
-      using finite_set_rel_transfer_back[OF 1 cs_rel_inv_single_valued] by simp
-  qed
-  lemma complement_3_language[simp]:
-    assumes "finite (nodes A)"
-    shows "language (complement_3 A) = streams (alphabet A) - language A"
-  proof -
-    have "(language (complement_3 A), language (complement_2 A)) \<in> \<langle>\<langle>Id\<rangle> stream_rel\<rangle> set_rel"
-      using complement_3_refine by parametricity auto
-    also have "(language (complement_2 A), language (complement_1 A)) \<in> \<langle>\<langle>Id\<rangle> stream_rel\<rangle> set_rel"
-      using complement_2_refine by parametricity auto
-    also have "(language (complement_1 A), language (complement A)) \<in> \<langle>\<langle>Id\<rangle> stream_rel\<rangle> set_rel"
-      using complement_1_refine by parametricity auto
-    also have "language (complement A) = streams (alphabet A) - language A"
-      using complement_language assms(1) by this
-    finally show "language (complement_3 A) = streams (alphabet A) - language A" by simp
-  qed
-
-(*
-  definition list_hash :: "('a :: hashable) list \<Rightarrow> uint32" where
-    "list_hash xs \<equiv> fold (bitXOR \<circ> hashcode) xs 0"
-*)
-
   definition "hci k \<equiv> uint32_of_nat k * 1103515245 + 12345"
   definition "hc \<equiv> \<lambda> (p, q, b). hci p + hci q * 31 + (if b then 1 else 0)"
   definition list_hash :: "(nat \<times> item) list \<Rightarrow> uint32" where
@@ -92,44 +57,31 @@ begin
   schematic_goal complement_impl:
     assumes [simp]: "finite (nodes A)"
     assumes [autoref_rules]: "(Ai, A) \<in> \<langle>Id, nat_rel\<rangle> nbai_nba_rel"
-    shows "(?f :: ?'c, RETURN (to_nbaei (complement_3 A))) \<in> ?R"
+    shows "(?f :: ?'c, RETURN (to_nbaei (complement_4 A))) \<in> ?R"
     by (autoref_monadic (plain))
   concrete_definition complement_impl uses complement_impl[unfolded autoref_tag_defs]
 
-  theorem
+  theorem complement_impl_correct:
     assumes "finite (nodes A)"
     assumes "(Ai, A) \<in> \<langle>Id, nat_rel\<rangle> nbai_nba_rel"
     shows "language (nbae_nba (nbaei_nbae (complement_impl Ai))) = streams (alphabet A) - language A"
   proof -
-    have "(language ((nbae_nba \<circ> nbaei_nbae) (complement_impl Ai)), language (id (complement_3 A))) \<in>
-      \<langle>\<langle>Id_on (alphabet (complement_3 A))\<rangle> stream_rel\<rangle> set_rel"
+    have "(language ((nbae_nba \<circ> nbaei_nbae) (complement_impl Ai)), language (id (complement_4 A))) \<in>
+      \<langle>\<langle>Id_on (alphabet (complement_4 A))\<rangle> stream_rel\<rangle> set_rel"
       using complement_impl.refine[OF assms, unfolded to_nbaei_def id_apply, THEN RETURN_nres_relD]
       by parametricity
-    also have "language (id (complement_3 A)) = streams (alphabet A) - language A"
-      using assms(1) by simp
+    also have "language (id (complement_4 A)) = streams (alphabet A) - language A"
+      using assms(1) complement_4_correct by simp
     finally show ?thesis by simp
   qed
 
-  definition s where
-    "s n a p \<equiv> if p = 0
-      then (if a = ''a'' then [0 ..< n] else [1])
-      else (if a = ''a'' then [1 ..< n] else [])"
-  definition "Ai n \<equiv> nbai [''a'', ''b''] [0] (s n) bot"
+  definition test :: "(String.literal, nat) nbaei \<Rightarrow> nat" where
+    "test A \<equiv> length (transei (complement_impl (nbae_nba_impl A)))"
 
-  definition "test n \<equiv> length (transei (complement_impl (Ai n)))"
-
-  (* TODO: maybe we can also do some crude optimizations about reachability *)
-  export_code complement_impl nat_of_integer integer_of_nat test
+  (* TODO: possible optimizations:
+    - introduce op_map_map operation for maps instead of manually iterating via FOREACH
+    - consolidate various binds and maps in expand_map_get_7 *)
+  export_code complement_impl nat_of_integer integer_of_nat test nbaei
     in SML module_name Complementation file "code/Complementation_Export.sml"
-
-  value "succi (complement_6 (Ai 3) 3) ''a'' (initiali (complement_6 (Ai 3) 3) ! 0) ! 7"
-  value "succi (complement_6 (Ai 3) 3) ''a'' (initiali (complement_6 (Ai 3) 3) ! 0) ! 27"
-  value "hashcode (1 :: nat, 1 :: nat, False)"
-  value "hashcode (0 :: nat, 0 :: nat, True)"
-  value "(1 :: nat) XOR 66"
-  value "hashcode (1 :: nat, 3 :: nat, False)"
-  value "hashcode (0 :: nat, 6 :: nat, True)"
-  value "(132 :: nat) XOR 199"
-  value "list_hash (succi (complement_6 (Ai 3) 3) ''a'' (initiali (complement_6 (Ai 3) 3) ! 0) ! 7)"
 
 end
